More attempt in quantifiers.

QuantifierLogic/ProofTheory/QuantifierLogic.v
@@ -1,27 +1,36 @@
 Require Import Logic.lib.Coqlib.
 Require Import Logic.GeneralLogic.Base.
 Require Import Logic.MinimunLogic.Syntax.
+Require Import Logic.QuantifierLogic.Syntax.
 Require Import Logic.MinimunLogic.ProofTheory.Normal.
 Require Import Logic.MinimunLogic.ProofTheory.Minimun.
 Require Import Logic.MinimunLogic.ProofTheory.RewriteClass.
 Require Import Logic.MinimunLogic.ProofTheory.ContextProperty.
-Require Import Logic.QuantifierLogic.Syntax.
 
 Local Open Scope logic_base.
 Local Open Scope syntax.
 
-Class QuantifierlLogic (BL: BinderLanguage) {nL: NormalLanguage _} {qL: QuantifierLanguage BL} (Gamma: ProofTheory _) {nGamma: NormalProofTheory _ Gamma} {mpGamma: MinimunPropositionalLogic _ Gamma} := {
-  allp_elim: forall (t: type) (x: binded_expr (t :: nil)) (e: term t),
+Class BindedProofTheory (BL: BinderLanguage): Type := {
+  binded_Gamma:> forall ts, ProofTheory (binded_L ts)
+}.
+
+Class QuantifierLogic
+      (BL: BinderLanguage)
+      {nL: forall ts, NormalLanguage (binded_L ts)}
+      {qL: QuantifierLanguage BL}
+      (BGamma: BindedProofTheory BL)
+      {nGamma: forall ts, NormalProofTheory (binded_L ts) (binded_Gamma ts)}
+      {mpGamma: forall ts, MinimunPropositionalLogic (binded_L ts) (binded_Gamma ts)} :=
+{
+  allp_elim: forall (t: type) (ts: list type) (x: binded_expr (t :: ts)) (e: term t),
     |-- allp x --> expr_instantiate x e;
-  allp_intros: forall (t: type) (x: expr) (y: binded_expr (t :: nil)) (e: term t),
-    is_const y ->
-    |-- x --> expr_instantiate y e ->
+  allp_gen: forall (t: type) (ts: list type) (x: binded_expr ts) (y: binded_expr (t :: ts)),
+    |-- (lift t x) --> y ->
     |-- x --> allp y;
-  exp_intros: forall (t: type) (x: binded_expr (t :: nil)) (e: term t),
+  exp_intros: forall (t: type) (ts: list type) (x: binded_expr (t :: ts)) (e: term t),
     |-- expr_instantiate x e --> exp x;
-  exp_elim: forall (t: type) (x: binded_expr (t :: nil)) (y: expr) (e: term t),
-    is_const x ->
-    |-- expr_instantiate x e --> y ->
+  exp_gen: forall (t: type) (ts: list type) (x: binded_expr (t :: ts)) (y: binded_expr ts),
+    |-- x --> lift t y ->
     |-- exp x --> y
 }.
 
