QuantifierLogic/Syntax.v
@@ -3,23 +3,22 @@ Require Import Logic.GeneralLogic.Base.
 Class BinderLanguage: Type := {
   type: Type;
   term: type -> Type;
-  binded_expr: list type -> Type;
-  expr_instantiate: forall (t0: type) (ts: list type), binded_expr (t0 :: ts) -> term t0 -> binded_expr ts
+  binded_L :> list type -> Language;
+  binded_expr := fun ts => @expr (binded_L ts);
+  expr_instantiate: forall (t: type) (ts: list type), binded_expr (t :: ts) -> term t -> binded_expr ts;
+  lift: forall (t: type) (ts: list type), binded_expr ts -> binded_expr (t :: ts);
+  lift_sound: forall (t: type) (ts: list type) (x: binded_expr ts) (e: term t), expr_instantiate t ts (lift t ts x) e = x
 }.
 
 Arguments binded_expr {_} _.
 Arguments expr_instantiate {_} {_} {_} _ _.
-
-Definition is_const {BL: BinderLanguage} {t: type} (x: binded_expr (t :: nil)): Prop :=
-  forall e1 e2, expr_instantiate x e1 = expr_instantiate x e2.
-
-Instance QuantifierLanguage2Language (BL: BinderLanguage): Language := Build_Language (binded_expr nil).
+Arguments lift {_} _ {_} _.
 
 Class QuantifierLanguage (BL: BinderLanguage): Type := {
-  allp: forall t, binded_expr (t :: nil) -> expr;
-  exp: forall t, binded_expr (t :: nil) -> expr
+  allp: forall t ts, binded_expr (t :: ts) -> binded_expr ts;
+  exp: forall t ts, binded_expr (t :: ts) -> binded_expr ts
 }.
 
-Arguments allp {_} {_} {_} _.
-Arguments exp {_} {_} {_} _.
+Arguments allp {_} {_} {_} {_} _.
+Arguments exp {_} {_} {_} {_} _.
 
