QuantifierLogic/ProofTheory/IntuitionisticDerivedRules.v
@@ -1,0 +1,54 @@
+Require Import Logic.lib.Coqlib.
+Require Import Logic.GeneralLogic.Base.
+Require Import Logic.MinimunLogic.Syntax.
+Require Import Logic.PropositionalLogic.Syntax.
+Require Import Logic.QuantifierLogic.Syntax.
+Require Import Logic.MinimunLogic.ProofTheory.Normal.
+Require Import Logic.MinimunLogic.ProofTheory.Minimun.
+Require Import Logic.MinimunLogic.ProofTheory.RewriteClass.
+Require Import Logic.MinimunLogic.ProofTheory.ContextProperty.
+Require Import Logic.PropositionalLogic.ProofTheory.Intuitionistic.
+Require Import Logic.QuantifierLogic.ProofTheory.QuantifierLogic.
+
+Local Open Scope logic_base.
+Local Open Scope syntax.
+Import PropositionalLanguageNotation.
+
+Lemma allp_K
+      (BL: BinderLanguage)
+      {nL: forall ts, NormalLanguage (binded_L ts)}
+      {pL: forall ts, PropositionalLanguage (binded_L ts)}
+      {qL: QuantifierLanguage BL}
+      (BGamma: BindedProofTheory BL)
+      {nGamma: forall ts, NormalProofTheory (binded_L ts) (binded_Gamma ts)}
+      {mpGamma: forall ts, MinimunPropositionalLogic (binded_L ts) (binded_Gamma ts)}
+      {ipGamma: forall ts, IntuitionisticPropositionalLogic (binded_L ts) (binded_Gamma ts)}
+      {qGamma: QuantifierLogic BL BGamma}:
+  forall (t: type) (ts: list type) (x y: binded_expr (t :: ts)),
+    |-- allp (x --> y) --> (allp x --> allp y).
+Proof.
+  intros.
+  rewrite provable_derivable.
+  rewrite <- !deduction_theorem.
+  eapply deduction_modus_ponens.
+  + apply deduction_andp_intros.
+    - apply derivable_assum1.
+    - apply deduction_weaken1.
+      apply derivable_assum1.
+  + apply deduction_weaken0.
+    eapply allp_gen.
+Abort.
+
+Lemma allp_intros
+      (BL: BinderLanguage)
+      {nL: forall ts, NormalLanguage (binded_L ts)}
+      {qL: QuantifierLanguage BL}
+      (BGamma: BindedProofTheory BL)
+      {nGamma: forall ts, NormalProofTheory (binded_L ts) (binded_Gamma ts)}
+      {mpGamma: forall ts, MinimunPropositionalLogic (binded_L ts) (binded_Gamma ts)}
+      {qGamma: QuantifierLogic BL BGamma}:
+  forall (t: type) (ts: list type) (x: binded_expr ts) (y: binded_expr (t :: ts)),
+    |-- allp (lift t x --> y) --> (x --> allp y).
+Proof.
+  intros.
+Abort.
